code/experimental/pkcs/Hacl.Impl.PKCS11.Creation.GenKey.fst
@@ -1,11 +1,24 @@
 module Hacl.Impl.PKCS11.Creation.GenKey
 
 open Hacl.Impl.PKCS11.Internal.Types
+open Hacl.Impl.PKCS11.Internal.Attribute
 open Hacl.Impl.PKCS11.DeviceModule
 
 open Hacl.Impl.PKCS11.Result
 
-(* C_GenerateKey generates a secret key or set of domain parameters, creating a new object. hSession is the session’s handle; pMechanism points to the generation mechanism; pTemplate points to the template for the new key or set of domain parameters; ulCount is the number of attributes in the template; phKey points to the location that receives the handle of the new key or set of domain parameters.
+open FStar.HyperStack.All
+open FStar.HyperStack
+module ST = FStar.HyperStack.ST
+
+open Lib.IntTypes
+open LowStar.Buffer
+
+(* C_GenerateKey generates a secret key or set of domain parameters, creating a new object. 
+hSession is the session’s handle; 
+pMechanism points to the generation mechanism; 
+pTemplate points to the template for the new key or set of domain parameters; 
+ulCount is the number of attributes in the template; 
+phKey points to the location that receives the handle of the new key or set of domain parameters.
 
 If the generation mechanism is for domain parameter generation, the CKA_CLASS attribute will have the value CKO_DOMAIN_PARAMETERS; otherwise, it will have the value CKO_SECRET_KEY.
 
@@ -15,7 +28,9 @@ If a call to C_GenerateKey cannot support the precise template supplied to it, i
 
 The object created by a successful call to C_GenerateKey will have its CKA_LOCAL attribute set to CK_TRUE.
 
-Return values: CKR_ARGUMENTS_BAD, CKR_ATTRIBUTE_READ_ONLY, CKR_ATTRIBUTE_TYPE_INVALID, CKR_ATTRIBUTE_VALUE_INVALID, CKR_CRYPTOKI_NOT_INITIALIZED, CKR_CURVE_NOT_SUPPORTED, CKR_DEVICE_ERROR, CKR_DEVICE_MEMORY, CKR_DEVICE_REMOVED, CKR_FUNCTION_CANCELED, CKR_FUNCTION_FAILED, CKR_GENERAL_ERROR, CKR_HOST_MEMORY, CKR_MECHANISM_INVALID, CKR_MECHANISM_PARAM_INVALID, CKR_OK, CKR_OPERATION_ACTIVE, CKR_PIN_EXPIRED, CKR_SESSION_CLOSED, CKR_SESSION_HANDLE_INVALID, CKR_SESSION_READ_ONLY, CKR_TEMPLATE_INCOMPLETE, CKR_TEMPLATE_INCONSISTENT, CKR_TOKEN_WRITE_PROTECTED, CKR_USER_NOT_LOGGED_IN.
+Return values: CKR_ARGUMENTS_BAD, 
+CKR_ATTRIBUTE_READ_ONLY -> val isAttributeReadOnly: _CK_ATTRIBUTE_TYPE -> Tot (r: exception_t {CKR_OK? r \/ CKR_ATTRIBUTE_READ_ONLY? r})
+CKR_ATTRIBUTE_TYPE_INVALID, CKR_ATTRIBUTE_VALUE_INVALID, CKR_CRYPTOKI_NOT_INITIALIZED, CKR_CURVE_NOT_SUPPORTED, CKR_DEVICE_ERROR, CKR_DEVICE_MEMORY, CKR_DEVICE_REMOVED, CKR_FUNCTION_CANCELED, CKR_FUNCTION_FAILED, CKR_GENERAL_ERROR, CKR_HOST_MEMORY, CKR_MECHANISM_INVALID, CKR_MECHANISM_PARAM_INVALID, CKR_OK, CKR_OPERATION_ACTIVE, CKR_PIN_EXPIRED, CKR_SESSION_CLOSED, CKR_SESSION_HANDLE_INVALID, CKR_SESSION_READ_ONLY, CKR_TEMPLATE_INCOMPLETE, CKR_TEMPLATE_INCONSISTENT, CKR_TOKEN_WRITE_PROTECTED, CKR_USER_NOT_LOGGED_IN.
 
 *)
 
@@ -24,6 +39,15 @@ val _CKS_GenerateKey:
   d: device -> 
   hSession: _CK_SESSION_HANDLE ->
   pMechanism: _CK_MECHANISM_TYPE ->
-  pTemplate: nat -> 
-  Tot 
+  ulCount: size_t -> 
+  pTemplate: buffer attribute {length pTemplate = uint_v ulCount} -> 
+  Stack 
     ((handler: result nat) & (device))
+    (requires fun h -> True)
+    (ensures fun h0 _ h1 -> True)
+
+
+let _CKS_GenerateKey d hSession pMechanism ulCould pTemplate = 
+  let testCall = checkAttributes ulCould pTemplate in 
+
+  (|Inl 0, d|) 
